Refactor

ML/plan_cert/src/mlunta_adapter.sml
@@ -6,6 +6,12 @@ Changes:
 structure MLuntaAdapter = struct
 open Mlunta
 
+fun parse_construct_and_check extra_lu net =
+    net
+    |> construct extra_lu
+    |> Either.mapR (snd #> (` Network.info))
+    |> Either.mapR (apsnd (` check_network))
+
 fun construct' extra_lu net =
     net
     |> Construction.construct extra_lu 
@@ -18,29 +24,29 @@ fun construct_and_check' extra_lu net =
     |> Either.mapR (apsnd (` check_network))
 
 val use_time' =
-    Benchmark.add_time (fn (time, res) => 
-        res
-        (* |> Either.mapL (fn err => (time, err))  *)
-        |> Either.mapR (fn succ => (time, succ))) 
+    Benchmark.add_time (fn (time, res) => Either.mapR (fn succ => (time, succ)) res) 
 
 fun check' extra_lu net =
     net
     |> Benchmark.time_it (construct_and_check' extra_lu)
     |> use_time'
     |> Either.mapR (fn (time, (info, (prop, net))) => (time, info, prop, net))
-(* 
-fun check_and_then' extra_lu post net =
+
+
+fun parse_check extra_lu net =
     net
-    |> Benchmark.time_it (construct_and_check' extra_lu)
-    |> use_time (fn time => fn (info, (prop, orig)) => (orig, post info time prop)) *)
+    |> Benchmark.time_it (parse_construct_and_check extra_lu)
+    |> use_time'
+    |> Either.mapR (fn (time, (info, (prop, net))) => (time, info, prop, net))
 
-fun compress' extra_lu compression net =
-    case net |> construct' extra_lu of
+fun compress' compression net =
+    case net of
         Either.Left _ => id
-    |   Either.Right (net, trans) => Comp.compress compression net trans
+    |   Either.Right (net, trans) => 
+        Comp.compress compression net trans
 
-fun certify' extra_lu version net =
-    case net |> construct' extra_lu of
+fun certify' version net =
+    case net of
         Either.Left _ => id
     |   Either.Right (net, trans) => fn x => (
         if Certify.check version net trans x
@@ -52,48 +58,70 @@ local
   open Formula
   open Property
 in
+    fun cert' compress certify time info result =
+        let
+            fun certs ht =
+                Diagnostic.make_with_cert time info ht
 
-fun cert' compress time info result =
-    let
-      fun certs ht =
-          Diagnostic.make_with_cert time info ht
-      val prop =
-          result |> the_formula |> just_prop
-    in
-      case result of
-          Ex (Unsatisfied ht) => 
-            let val ccert = compress ht
-            in (certs ccert prop, SOME ccert)
-            end |
-          Ag (Satisfied ht)   => 
-            let val ccert = compress ht
-            in (certs ccert prop, SOME ccert)
-            end |
-          _  => (Diagnostic.make_without_cert time prop, NONE)
-                    |> tap (K (Log.info "* No certificate extraction possible"))
-    end
+            val prop =
+                result |> the_formula |> just_prop
+
+            val no_certs =
+                Diagnostic.make_without_cert time prop
+        in
+        case result of
+            Ex (Unsatisfied ht) => 
+                let val ccert = ht |> compress |> certify
+                in (certs ccert prop, Either.Right ccert)
+                end |
+            Ag (Satisfied ht)   => 
+                let val ccert = ht |> compress |> certify
+                in (certs ccert prop, Either.Right ccert)
+                end |
+            Ex (Satisfied ht) => 
+                (no_certs, Either.Left ht)
+                |> tap (K (Log.info "* No certificate extraction possible")) |
+            Ag (Unsatisfied ht) => 
+                (no_certs, Either.Left ht) 
+                |> tap (K (Log.info "* No certificate extraction possible")) 
+        end
 end
 
-fun certc' compress renaming_path cert_path (time, info, prop, net) =
-    let val (res, ccert) = cert' compress time info prop
-        val _ = Diagnostic.finish (SOME (renaming_path, cert_path)) res
-    in ccert
-        |> Either.from_option ()
-        |> Either.mapR (fn states => (net, states))
+fun explore compress certify renaming_path cert_path (time, info, prop, net) =
+    let 
+        val (cont, explored) = cert' compress certify time info prop
+        val _ = cont |> Diagnostic.finish (SOME (renaming_path, cert_path))
+    in explored
+        |> Either.mapL (fn passed => (net, passed)) 
+        |> Either.mapR (fn passed => (net, passed))
     end
 
 fun check_and_cert_return extra_lu renaming_path cert_path net compression certification =
     net
     |> check' extra_lu
-    |> Either.bindR (
-        certc'
-            ((if compression > 0 then compress' extra_lu compression net else id) o
-                (if certification > 0 then certify' extra_lu certification net else id))
-            renaming_path 
+    |> Either.mapR (
+        explore
+            (if compression > 0 then compress' compression (construct' extra_lu net) else id)
+            (if certification > 0 then certify' certification (construct' extra_lu net) else id)
+            renaming_path
             cert_path)
 
 
 val check_and_cert_return_lu = check_and_cert_return true
 val check_and_cert_return = check_and_cert_return false
+
+fun parse_check_and_cert_return extra_lu renaming_path cert_path json_str compression certification =
+    json_str
+    |> parse_check extra_lu
+    |> Either.mapR (
+        explore
+            (if compression > 0 then compress' compression (construct extra_lu json_str) else id)
+            (if certification > 0 then certify' certification (construct extra_lu json_str) else id)
+            renaming_path 
+            cert_path)
+
+
+val parse_check_and_cert_return_lu = parse_check_and_cert_return true
+val parse_check_and_cert_return = parse_check_and_cert_return false
 
 end
