Makefile
@@ -1,0 +1,3 @@
+export_code:
+	isabelle build -d . -e PDDL_TP_Reduction
+.PHONY: export_code
